packaged ADT in a Module Type
--HG--
branch : adt

platform/cito/Semantics.v
@@ -1,51 +1,12 @@
-Require Import Syntax SemanticsExpr.
-Require Import IL Memory String Word Locals List.
-Require Import Label.
-
 Set Implicit Arguments.
 
-Record ADT := 
-  {
-    Model : Type
-  }.
+Require Import IL Memory String Locals List.
 
-Record ADTValue := 
-  {
-    Type_ : ADT;
-    Value : Model Type_
-  }.
-                    
-Variable Heap : Type.
-
-Variable heap_sel : Heap -> W -> option ADTValue.
-
-Variable heap_mem : W -> Heap -> Prop.
-
-Variable heap_upd : Heap -> W -> ADTValue -> Heap.
-
-Variable heap_remove : Heap -> W -> Heap.
-
-Variable heap_empty : Heap.
-
-Variable heap_merge : Heap -> Heap -> Heap.
-
-Variable heap_elements : Heap -> list (W * ADTValue).
-
-Variable heap_diff : Heap -> Heap -> Heap.
-
-Definition State := (vals * Heap)%type.
-
-Definition ArgIn := (W + ADTValue)%type.
-
-Definition ArgOut := option ADTValue.
-
-Definition Ret := (W + ADTValue)%type.
-
-Record ForeignFuncSpec := 
-  {
-    PreCond: list ArgIn -> Prop;
-    PostCond : list (ArgIn * ArgOut) -> Ret -> Prop
-  }.
+Definition upd_option vs x value :=
+  match x with
+    | None => vs
+    | Some s => Locals.upd vs s value
+  end.
 
 Require Import FuncCore.
 Export FuncCore.
@@ -57,126 +18,145 @@ Record InternalFuncSpec :=
 
 Coercion Fun : InternalFuncSpec >-> FuncCore.
 
-Inductive Callee := 
+Require Import ADT.
+
+Module Make (Import E : ADT).
+
+  Require Import Syntax SemanticsExpr.
+  Require Import Label.
+  Require Import Heap.
+  Module Import HeapMake := Heap.Make E.
+
+  Definition State := (vals * Heap)%type.
+
+  Definition ArgIn := (W + ADTValue)%type.
+
+  Definition ArgOut := option ADTValue.
+
+  Definition Ret := (W + ADTValue)%type.
+
+  Record ForeignFuncSpec := 
+    {
+      PreCond: list ArgIn -> Prop;
+      PostCond : list (ArgIn * ArgOut) -> Ret -> Prop
+    }.
+
+  Inductive Callee := 
   | Foreign : ForeignFuncSpec -> Callee
   | Internal : InternalFuncSpec -> Callee.
 
-Definition word_adt_match (heap : Heap) p :=
-  let word := fst p in
-  let in_ := snd p in
-  match in_ with
-    | inl w => word = w
-    | inr a => heap_sel heap word = Some a
-  end.
+  Definition word_adt_match (heap : Heap) p :=
+    let word := fst p in
+    let in_ := snd p in
+    match in_ with
+      | inl w => word = w
+      | inr a => heap_sel heap word = Some a
+    end.
 
-Definition is_adt (a : ArgIn) :=
-  match a with
-    | inl _ => false
-    | inr _ => true
-  end.
+  Definition is_adt (a : ArgIn) :=
+    match a with
+      | inl _ => false
+      | inr _ => true
+    end.
 
-Definition disjoint_ptrs (pairs : list (W * ArgIn)) := 
-  let pairs := filter (fun p => is_adt (snd p)) pairs in
-  NoDup (map fst pairs).
+  Definition disjoint_ptrs (pairs : list (W * ArgIn)) := 
+    let pairs := filter (fun p => is_adt (snd p)) pairs in
+    NoDup (map fst pairs).
 
-Definition good_inputs heap pairs := 
-  Forall (word_adt_match heap) pairs /\
-  disjoint_ptrs pairs.
+  Definition good_inputs heap pairs := 
+    Forall (word_adt_match heap) pairs /\
+    disjoint_ptrs pairs.
 
-Record ArgTriple :=
-  {
-    Word : W;
-    ADTIn : ArgIn;
-    ADTOut : ArgOut
-  }.
+  Record ArgTriple :=
+    {
+      Word : W;
+      ADTIn : ArgIn;
+      ADTOut : ArgOut
+    }.
 
-Fixpoint store_out (heap : Heap) t :=
-  match ADTIn t, ADTOut t with 
-    | inl _, _ => heap
-    | inr _, None => heap_remove heap (Word t)
-    | inr _, Some a => heap_upd heap (Word t) a
-  end.
+  Fixpoint store_out (heap : Heap) t :=
+    match ADTIn t, ADTOut t with 
+      | inl _, _ => heap
+      | inr _, None => heap_remove heap (Word t)
+      | inr _, Some a => heap_upd heap (Word t) a
+    end.
 
-Definition decide_ret addr (ret : Ret) :=
-  match ret with
-    | inl w => (w, None)
-    | inr a => (addr, Some a)
-  end.
+  Definition decide_ret addr (ret : Ret) :=
+    match ret with
+      | inl w => (w, None)
+      | inr a => (addr, Some a)
+    end.
 
-Definition separated heap ret_w (ret_a : option ADTValue) := 
-  ret_a = None \/ ~ heap_mem ret_w heap.
+  Definition separated heap ret_w (ret_a : option ADTValue) := 
+    ret_a = None \/ ~ heap_mem ret_w heap.
 
-Definition heap_upd_option m k v :=
-  match v with
-    | Some x => heap_upd m k x
-    | None => m
-  end.
+  Definition heap_upd_option m k v :=
+    match v with
+      | Some x => heap_upd m k x
+      | None => m
+    end.
 
-Definition upd_option vs x value :=
-  match x with
-    | None => vs
-    | Some s => Locals.upd vs s value
-  end.
+  (* Semantics *)
 
-(* Semantics *)
+  Section Env.
 
-Section Env.
+    Variable env : (label -> option W) * (W -> option Callee).
 
-  Variable env : (label -> option W) * (W -> option Callee).
+    Inductive RunsTo : Stmt -> State -> State -> Prop :=
+    | Skip : forall v, RunsTo Syntax.Skip v v
+    | Seq : 
+        forall a b v v' v'',
+          RunsTo a v v' -> 
+          RunsTo b v' v'' -> 
+          RunsTo (Syntax.Seq a b) v v''
+    | If : 
+        forall cond t f v v', 
+          let b := wneb (eval (fst v) cond) $0 in
+          b = true /\ RunsTo t v v' \/ b = false /\ RunsTo f v v' ->
+          RunsTo (Syntax.If cond t f) v v'
+    | While : 
+        forall cond body v v', 
+          let loop := While cond body in
+          RunsTo (Syntax.If cond (Syntax.Seq body loop) Syntax.Skip) v v' ->
+          RunsTo loop v v'
+    | CallInternal : 
+        forall var f args v spec vs_callee vs_callee' heap',
+          let vs := fst v in
+          let heap := snd v in
+          let fs := snd env in
+          fs (eval vs f) = Some (Internal spec) ->
+          map (Locals.sel vs_callee) (ArgVars spec) = map (eval vs) args ->
+          RunsTo (Body spec) (vs_callee, heap) (vs_callee', heap') ->
+          let vs := upd_option vs var (Locals.sel vs_callee' (RetVar spec)) in
+          let heap := heap' in
+          RunsTo (Syntax.Call var f args) v (vs, heap)
+    | CallForeign : 
+        forall var f args v spec triples addr ret,
+          let vs := fst v in
+          let heap := snd v in
+          let fs := snd env in
+          fs (eval vs f) = Some (Foreign spec) ->
+          map (eval vs) args = map Word triples ->
+          good_inputs heap (map (fun x => (Word x, ADTIn x)) triples) ->
+          PreCond spec (map ADTIn triples) ->
+          PostCond spec (map (fun x => (ADTIn x, ADTOut x)) triples) ret ->
+          let heap := fold_left store_out triples heap in
+          let t := decide_ret addr ret in
+          let ret_w := fst t in
+          let ret_a := snd t in
+          separated heap ret_w ret_a ->
+          let heap := heap_upd_option heap ret_w ret_a in
+          let vs := upd_option vs var ret_w in
+          RunsTo (Syntax.Call var f args) v (vs, heap)
+    | Label : 
+        forall x lbl v w,
+          fst env lbl = Some w ->
+          RunsTo (Syntax.Label x lbl) v (Locals.upd (fst v) x w, snd v)
+    | Assign :
+        forall x e v,
+          let vs := fst v in
+          RunsTo (Syntax.Assign x e) v (Locals.upd vs x (eval vs e), snd v).
 
-  Inductive RunsTo : Stmt -> State -> State -> Prop :=
-  | Skip : forall v, RunsTo Syntax.Skip v v
-  | Seq : 
-      forall a b v v' v'',
-        RunsTo a v v' -> 
-        RunsTo b v' v'' -> 
-        RunsTo (Syntax.Seq a b) v v''
-  | If : 
-      forall cond t f v v', 
-        let b := wneb (eval (fst v) cond) $0 in
-        b = true /\ RunsTo t v v' \/ b = false /\ RunsTo f v v' ->
-        RunsTo (Syntax.If cond t f) v v'
-  | While : 
-      forall cond body v v', 
-        let loop := While cond body in
-        RunsTo (Syntax.If cond (Syntax.Seq body loop) Syntax.Skip) v v' ->
-        RunsTo loop v v'
-  | CallInternal : 
-      forall var f args v spec vs_callee vs_callee' heap',
-        let vs := fst v in
-        let heap := snd v in
-        let fs := snd env in
-        fs (eval vs f) = Some (Internal spec) ->
-        map (Locals.sel vs_callee) (ArgVars spec) = map (eval vs) args ->
-        RunsTo (Body spec) (vs_callee, heap) (vs_callee', heap') ->
-        let vs := upd_option vs var (Locals.sel vs_callee' (RetVar spec)) in
-        let heap := heap' in
-        RunsTo (Syntax.Call var f args) v (vs, heap)
-  | CallForeign : 
-      forall var f args v spec triples addr ret,
-        let vs := fst v in
-        let heap := snd v in
-        let fs := snd env in
-        fs (eval vs f) = Some (Foreign spec) ->
-        map (eval vs) args = map Word triples ->
-        good_inputs heap (map (fun x => (Word x, ADTIn x)) triples) ->
-        PreCond spec (map ADTIn triples) ->
-        PostCond spec (map (fun x => (ADTIn x, ADTOut x)) triples) ret ->
-        let heap := fold_left store_out triples heap in
-        let t := decide_ret addr ret in
-        let ret_w := fst t in
-        let ret_a := snd t in
-        separated heap ret_w ret_a ->
-        let heap := heap_upd_option heap ret_w ret_a in
-        let vs := upd_option vs var ret_w in
-        RunsTo (Syntax.Call var f args) v (vs, heap)
-  | Label : 
-      forall x lbl v w,
-        fst env lbl = Some w ->
-        RunsTo (Syntax.Label x lbl) v (Locals.upd (fst v) x w, snd v)
-  | Assign :
-      forall x e v,
-        let vs := fst v in
-        RunsTo (Syntax.Assign x e) v (Locals.upd vs x (eval vs e), snd v).
+  End Env.
 
-End Env.
+End Make.
