platform/cito/Heap.v
@@ -1,0 +1,57 @@
+Set Implicit Arguments.
+
+Require Import Equalities.
+
+Module Key' <: MiniDecidableType.
+
+  Require Import Memory.
+
+  Definition t := W.
+
+  Require Import Word.
+
+  Definition eq_dec := @weq 32.
+
+End Key'.
+
+Module Key := Make_UDT Key'.
+
+Require Import ADT.
+
+Module Make (Import E : ADT).
+
+  Require Import FMapWeakList.
+
+  Module Import M := Make Key.
+
+  Definition elt := ADTValue.
+
+  Definition Heap := t elt.
+
+  Implicit Types m h : Heap.
+  Implicit Types x y z k p w : key.
+  Implicit Types e v a : elt.
+  Implicit Types ls : list (key * elt).
+
+  Definition heap_sel h p := find p h.
+
+  Definition heap_mem := @In elt.
+
+  Definition heap_upd h p v := add p v h.
+
+  Definition heap_remove h p := remove p h.
+
+  Definition heap_empty := @empty elt.
+
+  Require Import FMapFacts.
+
+  Module Import F := WFacts_fun Key M.
+  Module Import P := WProperties_fun Key M.
+
+  Definition heap_merge := @update elt.
+
+  Definition heap_elements := @elements elt.
+
+  Definition heap_diff := @diff elt.
+
+End Make.
