platform/cito/LayoutHints.v
@@ -7,12 +7,16 @@ Module Make (Import M : RepInv.RepInv).
 
   Module Import InvMake := Inv.Make M.
 
-  Lemma heap_empty_bwd : Emp ===> is_heap heap_empty.
-    admit.
-  Qed.
+  Section TopSection.
 
-  Definition hints_heap_empty_bwd : TacPackage.
-    prepare tt heap_empty_bwd.
-  Defined.
+    Lemma heap_empty_bwd : Emp ===> is_heap heap_empty.
+      admit.
+    Qed.
+
+    Definition hints_heap_empty_bwd : TacPackage.
+      prepare tt heap_empty_bwd.
+    Defined.
+
+  End TopSection.
 
 End Make.
