platform/cito/LayoutHints2.v
@@ -7,14 +7,18 @@ Module Make (Import M : RepInv.RepInv).
 
   Module Import InvMake := Inv.Make M.
 
-  Definition heap_to_split h (_ : list (W * ArgIn)) := is_heap h.
+  Section TopSection.
 
-  Lemma split_heap : forall h pairs, good_inputs h pairs -> heap_to_split h pairs ===> let h1 := make_heap pairs in is_heap h1 * is_heap (heap_diff h h1).
-    admit.
-  Qed.
+    Definition heap_to_split h (_ : list (W * ArgIn)) := is_heap h.
 
-  Definition hints_split_heap : TacPackage.
-    prepare split_heap tt.
-  Defined.
+    Lemma split_heap : forall h pairs, good_inputs h pairs -> heap_to_split h pairs ===> let h1 := make_heap pairs in is_heap h1 * is_heap (heap_diff h h1).
+      admit.
+    Qed.
+
+    Definition hints_split_heap : TacPackage.
+      prepare split_heap tt.
+    Defined.
+
+  End TopSection.
 
 End Make.
