platform/cito/LayoutHints3.v
@@ -7,28 +7,32 @@ Module Make (Import M : RepInv.RepInv).
 
   Module Import InvMake := Inv.Make M.
 
-  Definition is_heap_upd_option h addr a := is_heap (heap_upd_option h addr a).
+  Section TopSection.
 
-  Lemma is_heap_upd_option_bwd : forall h addr a, is_heap h * layout_option addr a ===> is_heap_upd_option h addr a.
-    admit.
-  Qed.
+    Definition is_heap_upd_option h addr a := is_heap (heap_upd_option h addr a).
 
-  Definition is_heap_merge h1 h2 := is_heap (heap_merge h1 h2).
+    Lemma is_heap_upd_option_bwd : forall h addr a, is_heap h * layout_option addr a ===> is_heap_upd_option h addr a.
+      admit.
+    Qed.
 
-  Lemma is_heap_merge_bwd : forall h1 h2, is_heap h1 * is_heap h2 ===> is_heap_merge h1 h2.
-    admit.
-  Qed.
+    Definition is_heap_merge h1 h2 := is_heap (heap_merge h1 h2).
 
-  Lemma star_merge_separated : forall specs st other h1 h2 addr adt, interp specs (![is_heap h1 * is_heap h2 * layout_option addr adt * other] st) -> separated (heap_merge h1 h2) addr adt.
-    admit.
-  Qed.
+    Lemma is_heap_merge_bwd : forall h1 h2, is_heap h1 * is_heap h2 ===> is_heap_merge h1 h2.
+      admit.
+    Qed.
 
-  Definition hints_heap_upd_option : TacPackage.
-    prepare tt is_heap_upd_option_bwd.
-  Defined.
+    Lemma star_merge_separated : forall specs st other h1 h2 addr adt, interp specs (![is_heap h1 * is_heap h2 * layout_option addr adt * other] st) -> separated (heap_merge h1 h2) addr adt.
+      admit.
+    Qed.
 
-  Definition hints_heap_merge : TacPackage.
-    prepare tt is_heap_merge_bwd.
-  Defined.
+    Definition hints_heap_upd_option : TacPackage.
+      prepare tt is_heap_upd_option_bwd.
+    Defined.
+
+    Definition hints_heap_merge : TacPackage.
+      prepare tt is_heap_merge_bwd.
+    Defined.
+
+  End TopSection.
 
 End Make.
