platform/cito/SemanticsFacts.v
@@ -1,54 +1,68 @@
-Require Import Semantics.
-Require Import Safe.
-Require Import SemanticsExpr.
-Require Import Notations.
+Set Implicit Arguments.
 
-Local Open Scope stmt.
+Require Import ADT.
 
-Lemma Safe_Seq_Skip : forall fs k v, Safe fs (skip ;; k) v -> Safe fs k v.
-  admit.
-Qed.
+Module Make (Import E : ADT).
 
-Lemma RunsTo_Seq_Skip : forall fs k v v', RunsTo fs k v v' -> RunsTo fs (skip ;; k) v v'.
-  admit.
-Qed.
+  Require Import Safe.
+  Module Import SafeMake := Safe.Make E.
+  Import SafeMake.SemanticsMake.
 
-Lemma Safe_Seq_assoc : forall fs a b c v, Safe fs ((a ;; b) ;; c) v -> Safe fs (a ;; b;; c) v.
-  admit.
-Qed.
+  Section TopSection.
 
-Lemma RunsTo_Seq_assoc : forall fs a b c v v', RunsTo fs (a ;; b ;; c) v v' -> RunsTo fs ((a ;; b) ;; c) v v'.
-  admit.
-Qed.
+    Require Import SemanticsExpr.
+    Require Import Notations.
 
-Lemma Safe_Seq_If_true : forall fs e t f k v, Safe fs (Syntax.If e t f ;; k) v -> wneb (eval (fst v) e) $0 = true -> Safe fs (t ;; k) v.
-  admit.
-Qed.
+    Local Open Scope stmt.
 
-Lemma RunsTo_Seq_If_true : forall fs e t f k v v', RunsTo fs (t ;; k) v v' -> wneb (eval (fst v) e) $0 = true -> RunsTo fs (Syntax.If e t f ;; k) v v'.
-  admit.
-Qed.
+    Lemma Safe_Seq_Skip : forall fs k v, Safe fs (skip ;; k) v -> Safe fs k v.
+      admit.
+    Qed.
 
-Lemma Safe_Seq_If_false : forall fs e t f k v, Safe fs (Syntax.If e t f ;; k) v -> wneb (eval (fst v) e) $0 = false -> Safe fs (f ;; k) v.
-  admit.
-Qed.
+    Lemma RunsTo_Seq_Skip : forall fs k v v', RunsTo fs k v v' -> RunsTo fs (skip ;; k) v v'.
+      admit.
+    Qed.
 
-Lemma RunsTo_Seq_If_false : forall fs e t f k v v', RunsTo fs (f ;; k) v v' -> wneb (eval (fst v) e) $0 = false -> RunsTo fs (Syntax.If e t f ;; k) v v'.
-  admit.
-Qed.
+    Lemma Safe_Seq_assoc : forall fs a b c v, Safe fs ((a ;; b) ;; c) v -> Safe fs (a ;; b;; c) v.
+      admit.
+    Qed.
 
-Lemma Safe_Seq_While_false : forall fs e s k v, Safe fs (Syntax.While e s ;; k) v -> wneb (eval (fst v) e) $0 = false -> Safe fs k v.
-  admit.
-Qed.
+    Lemma RunsTo_Seq_assoc : forall fs a b c v v', RunsTo fs (a ;; b ;; c) v v' -> RunsTo fs ((a ;; b) ;; c) v v'.
+      admit.
+    Qed.
 
-Lemma RunsTo_Seq_While_false : forall fs e s k v v', RunsTo fs k v v' -> wneb (eval (fst v) e) $0 = false -> RunsTo fs (Syntax.While e s ;; k) v v'.
-  admit.
-Qed.
+    Lemma Safe_Seq_If_true : forall fs e t f k v, Safe fs (Syntax.If e t f ;; k) v -> wneb (eval (fst v) e) $0 = true -> Safe fs (t ;; k) v.
+      admit.
+    Qed.
 
-Lemma Safe_Seq_While_true : forall fs e s k v, Safe fs (Syntax.While e s ;; k) v -> wneb (eval (fst v) e) $0 = true -> Safe fs (s ;; Syntax.While e s ;; k) v.
-  admit.
-Qed.
+    Lemma RunsTo_Seq_If_true : forall fs e t f k v v', RunsTo fs (t ;; k) v v' -> wneb (eval (fst v) e) $0 = true -> RunsTo fs (Syntax.If e t f ;; k) v v'.
+      admit.
+    Qed.
 
-Lemma RunsTo_Seq_While_true : forall fs e s k v v', RunsTo fs (s ;; Syntax.While e s ;; k) v v' -> wneb (eval (fst v) e) $0 = true -> RunsTo fs (Syntax.While e s ;; k) v v'.
-  admit.
-Qed.
+    Lemma Safe_Seq_If_false : forall fs e t f k v, Safe fs (Syntax.If e t f ;; k) v -> wneb (eval (fst v) e) $0 = false -> Safe fs (f ;; k) v.
+      admit.
+    Qed.
+
+    Lemma RunsTo_Seq_If_false : forall fs e t f k v v', RunsTo fs (f ;; k) v v' -> wneb (eval (fst v) e) $0 = false -> RunsTo fs (Syntax.If e t f ;; k) v v'.
+      admit.
+    Qed.
+
+    Lemma Safe_Seq_While_false : forall fs e s k v, Safe fs (Syntax.While e s ;; k) v -> wneb (eval (fst v) e) $0 = false -> Safe fs k v.
+      admit.
+    Qed.
+
+    Lemma RunsTo_Seq_While_false : forall fs e s k v v', RunsTo fs k v v' -> wneb (eval (fst v) e) $0 = false -> RunsTo fs (Syntax.While e s ;; k) v v'.
+      admit.
+    Qed.
+
+    Lemma Safe_Seq_While_true : forall fs e s k v, Safe fs (Syntax.While e s ;; k) v -> wneb (eval (fst v) e) $0 = true -> Safe fs (s ;; Syntax.While e s ;; k) v.
+      admit.
+    Qed.
+
+    Lemma RunsTo_Seq_While_true : forall fs e s k v v', RunsTo fs (s ;; Syntax.While e s ;; k) v v' -> wneb (eval (fst v) e) $0 = true -> RunsTo fs (Syntax.While e s ;; k) v v'.
+      admit.
+    Qed.
+
+  End TopSection.
+
+End Make.
