platform/cito/SemanticsFacts2.v
@@ -1,13 +1,26 @@
 Set Implicit Arguments.
 
-Require Import Semantics Safe.
-Require Import Notations.
-Local Open Scope stmt.
+Require Import ADT.
 
-Lemma Safe_Seq_Skip_Safe : forall fs s v, Safe fs s v -> Safe fs (s ;; skip) v.
-  admit.
-Qed.
+Module Make (Import E : ADT).
 
-Lemma RunsTo_Seq_Skip_RunsTo : forall fs s v v', RunsTo fs (s ;; skip) v v' -> RunsTo fs s v v'.
-  admit.
-Qed.
+  Require Import Safe.
+  Module Import SafeMake := Safe.Make E.
+  Import SafeMake.SemanticsMake.
+
+  Section TopSection.
+
+    Require Import Notations.
+    Local Open Scope stmt.
+
+    Lemma Safe_Seq_Skip_Safe : forall fs s v, Safe fs s v -> Safe fs (s ;; skip) v.
+      admit.
+    Qed.
+
+    Lemma RunsTo_Seq_Skip_RunsTo : forall fs s v v', RunsTo fs (s ;; skip) v v' -> RunsTo fs s v v'.
+      admit.
+    Qed.
+
+  End TopSection.
+
+End Make.
