platform/cito/SepHints5.v
@@ -2,50 +2,54 @@ Require Import SepHints2.
 
 Set Implicit Arguments.
 
-Lemma split_buf : forall p len pos, buf_splittable len pos -> buf_to_split p len pos ===> p =?> pos * (p ^+ $(4 * pos)) =?> (len - pos).
-  admit.
-Qed.
+Section TopSection.
 
-Definition hints_split_buf : TacPackage.
-  prepare split_buf tt.
-Defined.
+  Lemma split_buf : forall p len pos, buf_splittable len pos -> buf_to_split p len pos ===> p =?> pos * (p ^+ $(4 * pos)) =?> (len - pos).
+    admit.
+  Qed.
 
-Definition to_intro_array (_ : W) := True.
+  Definition hints_split_buf : TacPackage.
+    prepare split_buf tt.
+  Defined.
 
-Lemma intro_array : forall len p, to_intro_array p -> p =?> len ===> Ex ls, [| length ls = len |] * array ls p.
-  admit.
-Qed.
+  Definition to_intro_array (_ : W) := True.
 
-Definition combined_locals vars1 vars2 vs1 vs2 p  := locals (vars1 ++ vars2) (merge vs1 vs2 vars1) 0 p.
+  Lemma intro_array : forall len p, to_intro_array p -> p =?> len ===> Ex ls, [| length ls = len |] * array ls p.
+    admit.
+  Qed.
 
-Lemma fold_combined_locals : forall vars1 vars2 vs1 vs2 p, locals (vars1 ++ vars2) (merge vs1 vs2 vars1) 0 p = combined_locals vars1 vars2 vs1 vs2 p.
-  eauto.
-Qed.
+  Definition combined_locals vars1 vars2 vs1 vs2 p  := locals (vars1 ++ vars2) (merge vs1 vs2 vars1) 0 p.
 
-Definition locals_combinable A (vars vars2 : list A) := NoDup (vars ++ vars2).
+  Lemma fold_combined_locals : forall vars1 vars2 vs1 vs2 p, locals (vars1 ++ vars2) (merge vs1 vs2 vars1) 0 p = combined_locals vars1 vars2 vs1 vs2 p.
+    eauto.
+  Qed.
 
-Lemma combine_locals : forall vars1 vars2 vs1 vs2 p, locals vars1 vs1 0 p * locals vars2 vs2 0 (p ^+ $(4 * length vars1)) ===> combined_locals vars1 vars2 vs1 vs2 p.
-  admit.
-Qed.
+  Definition locals_combinable A (vars vars2 : list A) := NoDup (vars ++ vars2).
 
-Definition hints_intro_array : TacPackage.
-  prepare intro_array tt.
-Defined.
+  Lemma combine_locals : forall vars1 vars2 vs1 vs2 p, locals vars1 vs1 0 p * locals vars2 vs2 0 (p ^+ $(4 * length vars1)) ===> combined_locals vars1 vars2 vs1 vs2 p.
+    admit.
+  Qed.
 
-Definition hints_combine_locals : TacPackage.
-  prepare tt combine_locals.
-Defined.
+  Definition hints_intro_array : TacPackage.
+    prepare intro_array tt.
+  Defined.
 
-Definition locals_to_split vars1 vars2 vs p := locals (vars1 ++ vars2) vs 0 p.
+  Definition hints_combine_locals : TacPackage.
+    prepare tt combine_locals.
+  Defined.
 
-Lemma fold_locals_to_split : forall vars1 vars2 vs p, locals (vars1 ++ vars2) vs 0 p = locals_to_split vars1 vars2 vs p.
-  eauto.
-Qed.
+  Definition locals_to_split vars1 vars2 vs p := locals (vars1 ++ vars2) vs 0 p.
 
-Lemma split_locals : forall vars1 vars2 vs p, locals_to_split vars1 vars2 vs p ===> locals vars1 vs 0 p * locals vars2 vs 0 (p ^+ $(4 * length vars1)).
-  admit.
-Qed.
+  Lemma fold_locals_to_split : forall vars1 vars2 vs p, locals (vars1 ++ vars2) vs 0 p = locals_to_split vars1 vars2 vs p.
+    eauto.
+  Qed.
 
-Definition hints_split_locals : TacPackage.
-  prepare split_locals tt.
-Defined.
+  Lemma split_locals : forall vars1 vars2 vs p, locals_to_split vars1 vars2 vs p ===> locals vars1 vs 0 p * locals vars2 vs 0 (p ^+ $(4 * length vars1)).
+    admit.
+  Qed.
+
+  Definition hints_split_locals : TacPackage.
+    prepare split_locals tt.
+  Defined.
+
+End TopSection.
